wip

Logic/Propositional/Intuitionistic/Kripke/Completeness.lean
@@ -5,6 +5,8 @@ namespace LO.Propositional.Intuitionistic
 
 open Formula Theory Kripke
 open Hilbert
+open Set
+
 
 section Consistency
 
@@ -18,14 +20,21 @@ lemma consistent_subset_undeducible_falsum (hΔ : Δ ⊆ Γ) : (Δ ⊬ᴵ! ⊥) 
 
 lemma consistent_neither_undeducible : (Γ ⊬ᴵ! p) ∨ (Γ ⊬ᴵ! ~p) := Hilbert.consistent_neither_undeducible (· ⊢ᴵ ·) hConsisΓ p
 
+lemma consistent_of_undeducible : (Γ ⊬ᴵ! p) → Consistent Γ := by
+  intros;
+  simp [consistent_iff_undeducible_falsum];
+  by_contra hC;
+  have : Γ ⊢ᴵ! p := efq'! (by simpa [Undeducible] using hC);
+  contradiction;
+
 end Consistency
 
 
 namespace Theory
 
-def Closed (Γ : Theory β) := ∀ p, (Γ ⊢ᴵ! p) → (p ∈ Γ)
+def Closed (Γ : Theory β) := ∀ {p}, (Γ ⊢ᴵ! p) → (p ∈ Γ)
 
-def Disjunctive (Γ : Theory β) := ∀ p q, (p ⋎ q ∈ Γ) → (p ∈ Γ) ∨ (q ∈ Γ)
+def Disjunctive (Γ : Theory β) := ∀ {p q}, (p ⋎ q ∈ Γ) → (p ∈ Γ) ∨ (q ∈ Γ)
 
 class Prime (T : Theory β) where
   consistent : Consistent T
@@ -40,17 +49,23 @@ structure PrimeTheory (β) where
 
 namespace PrimeTheory
 
-variable (Ω : PrimeTheory β)
-
-def consistent : Consistent Ω.theory := Ω.prime.consistent
-def closed : Closed Ω.theory := Ω.prime.closed
-def disjunctive : Disjunctive Ω.theory := Ω.prime.disjunctive
-
 @[simp] def membership (p : Formula β) (Ω : PrimeTheory β) := p ∈ Ω.theory
 instance : Membership (Formula β) (PrimeTheory β) := ⟨membership⟩
 
 @[simp] def subset (Ω₁ Ω₂ : PrimeTheory β) := Ω₁.theory ⊆ Ω₂.theory
 instance : HasSubset (PrimeTheory β) := ⟨subset⟩
+
+variable (Ω : PrimeTheory β)
+
+def consistent : Consistent Ω.theory := Ω.prime.consistent
+
+def closed : Closed Ω.theory := Ω.prime.closed
+
+lemma closed' {p : Formula β} : (Ω.theory ⊢ᴵ! p) → (p ∈ Ω) := Ω.closed p
+
+def disjunctive : Disjunctive Ω.theory := Ω.prime.disjunctive
+
+lemma disjunctive' {p q : Formula β} : (p ⋎ q ∈ Ω) → (p ∈ Ω) ∨ (q ∈ Ω) := Ω.disjunctive p q
 
 variable {Ω}
 
@@ -58,100 +73,177 @@ variable {Ω}
 
 @[simp] lemma no_falsum : ⊥ ∉ Ω := consistent_no_falsum Ω.consistent
 
-lemma closed' {p : Formula β} : (Ω.theory ⊢ᴵ! p) → (p ∈ Ω) := Ω.closed p
-lemma disjunctive' {p q : Formula β} : (p ⋎ q ∈ Ω) → (p ∈ Ω) ∨ (q ∈ Ω) := Ω.disjunctive p q
-
 end PrimeTheory
 
-section PrimeExpand
+section
 
-variable [Encodable (Formula β)]
 open Encodable
+open Classical
 
--- variable [∀ (Γ : Theory β) (p : Formula β), Decidable (Γ ⊢ᴵ! p)]
-
-open Classical in
-@[simp] def primex_next (Γ : Theory β) (p : Formula β) (n : ℕ) : Theory β :=
-  match (decode n) with
-  | some (q₁ ⋎ q₂ : Formula β) =>
-    if Γ ⊢ᴵ! (q₁ ⋎ q₂)
-      then if (insert q₁ Γ) ⊢ᴵ! p then insert q₂ Γ else insert q₁ Γ
-      else Γ
-  | _ => Γ
-
-def primex_family (Γ : Theory β) (p : Formula β) : ℕ → Theory β
-  | 0 => Γ
-  | n + 1 => primex_next Γ p n
-
-notation Γ "[" p "," i "]" => primex_family Γ p i
+variable {Γ : Theory β} {p : Formula β} (hD : Γ ⊬ᴵ! p)
+variable [Encodable (Formula β)]
 
 @[simp]
-lemma def_primex_family_zero (Γ : Theory β) : Γ[p, 0] = Γ := rfl
+def insert_family (Γ : Theory β) (p : Formula β) : ℕ → Theory β
+  | 0 => Γ
+  | n + 1 =>
+    match (decode n) with
+    | some (q : Formula β) =>
+      match q with
+      | q₁ ⋎ q₂ =>
+        if (insert_family Γ p n) ⊢ᴵ! (q₁ ⋎ q₂)
+          then if (insert q₁ (insert_family Γ p n)) ⊢ᴵ! p
+            then insert q₂ (insert_family Γ p n)
+            else insert q₁ (insert_family Γ p n)
+          else (insert_family Γ p n)
+      | _ => insert_family Γ p n
+    | _ => insert_family Γ p n
+notation Γ "[" p "," i "]ᴵ" => insert_family Γ p i
 
-lemma primex_family_closed {Γ : Theory β} (h : Closed Γ) {p i} : Closed (Γ[p, i]) := by
-  induction i with
-  | zero => simp [primex_family]; simpa;
-  | succ i ih =>
-    simp_all [Closed];
-    intro q hq;
-    have := h q;
-    have := ih q;
-    sorry;
 
-lemma primex_family_disjunctive {Γ : Theory β} (h : Disjunctive Γ) {p i} : Disjunctive (Γ[p, i]) := by
-  induction i with
-  | zero => simp [primex_family]; simpa;
-  | succ i ih => sorry;
-
-lemma subset_primex_family_original {Γ : Theory β} {p i} : Γ ⊆ Γ[p, i] := by
-  induction i with
-  | zero => simp [primex_family]; rfl
-  | succ =>
-    simp [primex_family];
-    split; split; split;
-    all_goals (first | simp | rfl);
-
-lemma primex_family_subset_succ {Γ : Theory β} {p i} : Γ[p, i] ⊆ Γ[p, i + 1] := by
-  induction i with
-  | zero =>
-    simp [primex_family];
-    split; split; split;
-    all_goals (first | simp | rfl);
-  | succ k ih => sorry;
-
-lemma primex_family_subset_monotone {Γ : Theory β} {p i j} (h : i ≤ j) : Γ[p, i] ⊆ Γ[p, j] := by
+lemma insert_family_mono (h : k ≤ m) : Γ[p, k]ᴵ ⊆ Γ[p, m]ᴵ := by
   induction h with
-  | refl => rfl
-  | step _ ih => exact Set.Subset.trans ih primex_family_subset_succ
-
-lemma primex_family_monotone (Γ : Theory β) (p : Formula β) : Monotone (Γ[p, ·]) := by
-  intro _ _ h; exact primex_family_subset_monotone h
-
-def primex_family_sets (Γ : Theory β) (p : Formula β) : Set (Theory β) := { Γ[p, i] | i : ℕ }
-
-lemma exists_primex (Γ : Theory β) (p : Formula β)
-  : ∃ m ∈ { Γ[p, i] | i : ℕ }, Γ ⊆ m ∧ ∀ a ∈ { Γ[p, i] | i : ℕ }, m ⊆ a → a = m
-  := zorn_subset_nonempty { Γ[p, i] | i : ℕ } (by
-    intro c hc chain hnc;
-    existsi (⋃₀ c);
+  | refl => rfl;
+  | step h ih =>
     simp;
-    constructor;
-    . by_contra hC; simp at hC; sorry;
-    . intro s a;
-      exact Set.subset_sUnion_of_mem a;
-  ) Γ (by existsi 0; simp)
+    split;
+    . split;
+      . split;
+        . split;
+          apply Set.Subset.trans ih; aesop;
+          apply Set.Subset.trans ih; aesop;
+        . simpa;
+      . simpa;
+    . simpa;
 
-noncomputable def primex (Γ : Theory β) (p : Formula β) : Theory β := exists_primex Γ p |>.choose
-notation Γ "[" p "]" => primex Γ p
+lemma insert_family_subset_self : Γ ⊆ Γ[p, k]ᴵ := insert_family_mono (zero_le k)
 
-lemma primeExpand {Γ : Theory β} (hp : Γ ⊬ᴵ! p) : ∃ Ω : PrimeTheory β, (Γ ⊆ Ω.theory ∧ Ω.theory ⊬ᴵ! p) := by
-  have ⟨Ω, ⟨h₁, ⟨h₂, h₃⟩⟩⟩ := exists_primex Γ ⊥;
-  existsi ⟨Ω, (by sorry), (by sorry), (by sorry)⟩
+lemma insert_family_undeducible : ∀ {i}, Γ[p, i]ᴵ ⊬ᴵ! p := by
+  intro i;
+  induction i with
+  | zero => simpa;
+  | succ i ih =>
+    simp;
+    cases @decode (Formula β) _ i with
+    | none => simpa;
+    | some q =>
+      simp;
+      split;
+      . split;
+        . split;
+          . rename_i q₁ q₂ hq₁₂ hq₁;
+            by_contra hq₂;
+            replace hq₁ : Γ[p,i]ᴵ ⊢ᴵ! (q₁ ⟶ p) := dtr! (by simpa [Undeducible] using hq₁);
+            replace hq₂ : Γ[p,i]ᴵ ⊢ᴵ! (q₂ ⟶ p) := dtr! (by simpa [Undeducible] using hq₂);
+            have : Γ[p,i]ᴵ ⊢ᴵ! p := disj₃'! hq₁ hq₂ hq₁₂;
+            contradiction;
+          . simpa;
+        . simpa;
+      . simpa;
+
+lemma insert_family_deducible : (Γ[p, i]ᴵ ⊢ᴵ! p) → (Γ ⊢ᴵ! p) := by
+  contrapose;
+  intro h;
+  exact insert_family_undeducible h
+
+@[simp]
+def prime_family (Γ : Theory β) (p : Formula β) : ℕ → Theory β
+  | 0 => Γ
+  | n + 1 => ⋃ i, (prime_family Γ p n)[p, i]ᴵ
+notation Γ "[" p "," i "]ᴾ" => prime_family Γ p i
+
+lemma prime_family_mono (h : k ≤ m) : Γ[p, k]ᴾ ⊆ Γ[p, m]ᴾ := by
+  induction h with
+  | refl => rfl;
+  | @step m _ ih =>
+    apply Subset.trans ih;
+    nth_rw 1 [(show Γ[p, m]ᴾ = (Γ[p, m]ᴾ)[p, 0]ᴵ by rfl)];
+    apply subset_iUnion;
+
+lemma insert_family_deducible_of_prime_family_deducible (h : Γ[p, k + 1]ᴾ ⊢ᴵ! p) : ∃ m, (Γ[p, k]ᴾ[p, m]ᴵ ⊢ᴵ! p) := by
+  sorry;
+
+lemma prime_family_deducible : (Γ[p, k]ᴾ ⊢ᴵ! p) → (Γ ⊢ᴵ! p) := by
+  induction k with
+  | zero => simp;
+  | succ k ih =>
+    intro h;
+    obtain ⟨m, hm⟩ := insert_family_deducible_of_prime_family_deducible h;
+    exact ih (insert_family_deducible hm);
+
+lemma prime_family_undeducible : Γ ⊬ᴵ! p → ∀ {k}, Γ[p, k]ᴾ ⊬ᴵ! p := by
+  contrapose;
+  intro h;
+  obtain ⟨k, (hk : Γ[p, k]ᴾ ⊢ᴵ! p)⟩ := by simpa [Undeducible] using h;
+  simpa [Undeducible] using prime_family_deducible hk;
+
+@[simp]
+def prime_family_union (Γ : Theory β) (p : Formula β) : Theory β := ⋃ i, Γ[p, i]ᴾ
+notation Γ "[" p "]ᴾ" => prime_family_union Γ p
+
+lemma mem_prime_family_union (h : q ∈ (Γ[p, m]ᴾ)[p, k]ᴵ) : q ∈ Γ[p]ᴾ := by
+  simp;
+  existsi (m + 1);
+  simp;
+  existsi k;
+  simpa;
+
+lemma prime_family_union_disjunctive : Disjunctive (Γ[p]ᴾ) := by
+  intros q₁ q₂ hq;
+  let k := encode (q₁ ⋎ q₂);
+  obtain ⟨m, hm⟩ := by simpa using hq;
+  have hm₀ : (Γ[p, m]ᴾ)[p, 0]ᴵ ⊢ᴵ! q₁ ⋎ q₂ := by simpa using axm! hm;
+  have hmₖ : (Γ[p, m]ᴾ)[p, k]ᴵ ⊢ᴵ! q₁ ⋎ q₂ := weakening! (insert_family_mono (zero_le k)) hm₀;
+  have h : q₁ ∈ (Γ[p, m]ᴾ)[p, k + 1]ᴵ ∨ q₂ ∈ (Γ[p, m]ᴾ)[p, k + 1]ᴵ := by
+    simp [k, hmₖ];
+    split;
+    . right; simp;
+    . left; simp;
+  cases h with
+  | inl h => left; apply mem_prime_family_union h;
+  | inr h => right; apply mem_prime_family_union h;
+
+lemma exists_prime_family_union_deducible : Γ[p]ᴾ ⊢ᴵ! q → ∃ k, Γ[p, k]ᴾ ⊢ᴵ! q := by
+  sorry;
+
+lemma prime_family_union_closed : Closed (Γ[p]ᴾ) := by
+  intro q hq;
+  let k := encode (p ⋎ q);
+  have hpq : Γ[p]ᴾ ⊢ᴵ! (p ⋎ q) := disj₂'! hq;
+  obtain ⟨m, hm⟩ := exists_prime_family_union_deducible hpq;
+  have hm₀ : (Γ[p, m]ᴾ)[p, 0]ᴵ ⊢ᴵ! p ⋎ q := by simpa;
+  have hmₖ : (Γ[p, m]ᴾ)[p, k]ᴵ ⊢ᴵ! p ⋎ q := weakening! (insert_family_mono (zero_le k)) hm₀;
+  have h : q ∈ (Γ[p, m]ᴾ)[p, k + 1]ᴵ := by simp [k, hmₖ, axm!];
+  exact mem_prime_family_union h;
+
+lemma prime_family_union_undeducible : Γ[p]ᴾ ⊬ᴵ! p := by
+  by_contra hC;
+  replace hC : Γ[p]ᴾ ⊢ᴵ! p := by simpa [Undeducible] using hC;
+  obtain ⟨m, (hm : Γ[p, m]ᴾ ⊢ᴵ! p)⟩ := exists_prime_family_union_deducible hC;
+  have : Γ[p, m]ᴾ ⊬ᴵ! p := prime_family_undeducible hD;
+  contradiction;
+
+lemma prime_family_union_consistent : Theory.Consistent (Γ[p]ᴾ) := by
+  by_contra hC;
+  replace hC : Γ[p]ᴾ ⊢ᴵ! ⊥ := by simpa [Undeducible] using hC;
+  have : Γ[p]ᴾ ⊬ᴵ! p := prime_family_union_undeducible hD;
+  have : Γ[p]ᴾ ⊢ᴵ! p := efq'! hC;
+  contradiction;
+
+lemma prime_family_union_subset_self : Γ ⊆ Γ[p]ᴾ := by
+  intro q hq;
+  simp [prime_family_union];
+  existsi 0;
+  simpa;
+
+lemma prime_expansion : ∃ Ω : PrimeTheory β, (Γ ⊆ Ω.theory ∧ Ω.theory ⊬ᴵ! p) := by
+  let Ω : PrimeTheory β := ⟨Γ[p]ᴾ, ⟨prime_family_union_consistent hD, prime_family_union_closed, prime_family_union_disjunctive⟩⟩;
+  existsi Ω;
   constructor;
-  . exact h₂;
-  . sorry; -- exact h₃;
+  . apply prime_family_union_subset_self;
+  . apply prime_family_union_undeducible hD;
 
-end PrimeExpand
+end
 
 variable [Encodable (Formula β)] -- TODO: remove
 
@@ -205,7 +297,7 @@ lemma truthlemma {Ω : PrimeTheory β} {p : Formula β} : (Ω ⊩[(CanonicalMode
       intro h;
       simp [KripkeSatisfies.imp_def'];
       have h₁ : insert p Ω.theory ⊬ᴵ! q := dtr_not! h;
-      obtain ⟨Ω', hΩ'₁, hΩ'₂⟩ := primeExpand h₁;
+      obtain ⟨Ω', hΩ'₁, hΩ'₂⟩ := prime_expansion h₁;
       existsi Ω';
       exact ⟨
         ihp.mpr $ axm! (by aesop),
@@ -226,7 +318,7 @@ lemma truthlemma {Ω : PrimeTheory β} {p : Formula β} : (Ω ⊩[(CanonicalMode
 lemma Kripke.completes {Γ : Theory β} {p : Formula β} : (Γ ⊨ᴵ p) → (Γ ⊢ᴵ! p) := by
   contrapose;
   intro hnp hp;
-  have ⟨Ω, ⟨hsΩ, hnpΩ⟩⟩ := primeExpand hnp;
+  have ⟨Ω, ⟨hsΩ, hnpΩ⟩⟩ := prime_expansion hnp;
   have := truthlemma.not.mpr hnpΩ;
   have := hp (CanonicalModel β) Ω (by
     intro q hq;
